books/centaur/fgl/interp.lisp
@@ -30,6 +30,7 @@
 
 (in-package "FGL")
 
+(include-book "interp-st")
 (include-book "bvar-db-equivs")
 (include-book "bfr-arithmetic")
 (include-book "glcp-unify-defs")
@@ -53,13 +54,28 @@
 ;;                   (not (member bfr (gl-object-bfrlist val))))
 ;;              (not (member bfr (glcp-unify-alist-bfrlist (cons (cons key val) x)))))))
 
-(define glcp-interp-error (msg &key (interp-st 'interp-st)
-                               (state 'state))
-  :returns (mv errmsg
-               result
-               new-interp-st
-               new-state)
-  (mv msg nil interp-st state))
+;; Trace this!
+(define glcp-interp-error-message ((str stringp)
+                                   (arglist))
+  :returns (error-message (or (consp error-message)
+                              (stringp error-message))
+                          :rule-classes :type-prescription)
+  (if arglist
+      (cons (str-fix str) arglist)
+    (str-fix str)))
+
+(defmacro gl-msg (str &rest args)
+  `(glcp-interp-error-message ,str ,(make-fmt-bindings acl2::*base-10-chars* args)))
+
+
+
+;; (define glcp-interp-error (msg &key (interp-st 'interp-st)
+;;                                (state 'state))
+;;   :returns (mv errmsg
+;;                result
+;;                new-interp-st
+;;                new-state)
+;;   (mv msg nil interp-st state))
 
 (defmacro glcp-value (obj)
   `(mv nil ,obj interp-st state))
@@ -74,9 +90,168 @@
     :g-apply t
     :otherwise nil))
 
-(define interp-st->stack-top (interp-st)
+
+(define interp-st-bindings (interp-st)
   :enabled t
-  (car (interp-st->stack interp-st)))
+  :inline t
+  (stobj-let ((stack (interp-st->stack interp-st)))
+             (bindings)
+             (stack-bindings stack)
+             bindings))
+
+(define interp-st-stack-len (interp-st)
+  :enabled t
+  :inline t
+  (stobj-let ((stack (interp-st->stack interp-st)))
+             (len)
+             (stack-len stack)
+             len))
+
+(define interp-st-pop-frame (interp-st)
+  :enabled t
+  :inline t
+  :guard (< 1 (interp-st-stack-len interp-st))
+  (stobj-let ((stack (interp-st->stack interp-st)))
+             (stack)
+             (stack-pop-frame stack)
+             interp-st))
+
+(define interp-st-push-scratch ((x gl-object-p)
+                                interp-st)
+  :enabled t
+  :inline t
+  :guard (< 1 (interp-st-stack-len interp-st))
+  (stobj-let ((stack (interp-st->stack interp-st)))
+             (stack)
+             (stack-push-scratch x stack)
+             interp-st))
+
+(define interp-st-scratch-len (interp-st)
+  :enabled t
+  :inline t
+  (stobj-let ((stack (interp-st->stack interp-st)))
+             (len)
+             (stack-scratchlen stack)
+             len))
+
+(define interp-st-pop-scratch ((n natp)
+                                interp-st)
+  :enabled t
+  :inline t
+  :guard (<= n (interp-st-scratch-len interp-st))
+  (stobj-let ((stack (interp-st->stack interp-st)))
+             (stack)
+             (stack-pop-scratch n stack)
+             interp-st))
+
+(define interp-st-peek-scratch ((n natp)
+                                interp-st)
+  :enabled t
+  :inline t
+  :guard (<= n (interp-st-scratch-len interp-st))
+  (stobj-let ((stack (interp-st->stack interp-st)))
+             (args)
+             (stack-peek-scratch n stack)
+             args))
+
+(define interp-st-add-bindings ((x gl-object-alist-p)
+                                interp-st)
+  :enabled t
+  :inline t
+  (stobj-let ((stack (interp-st->stack interp-st)))
+             (stack)
+             (stack-add-bindings x stack)
+             interp-st))
+
+(define interp-st-set-bindings ((x gl-object-alist-p)
+                                interp-st)
+  :enabled t
+  :inline t
+  (stobj-let ((stack (interp-st->stack interp-st)))
+             (stack)
+             (stack-set-bindings x stack)
+             interp-st))
+
+(define interp-st-push-frame ((bindings gl-object-alist-p)
+                              interp-st)
+  :enabled t
+  :inline t
+  (stobj-let ((stack (interp-st->stack interp-st)))
+             (stack)
+             (b* ((stack (stack-push-frame stack)))
+               (stack-set-bindings bindings stack))
+             interp-st))
+
+(define interp-st-dup-frame (interp-st)
+  :enabled t
+  :inline t
+  (stobj-let ((stack (interp-st->stack interp-st)))
+             (stack)
+             (b* ((bindings (stack-bindings stack))
+                  (stack (stack-push-frame stack)))
+               (stack-set-bindings bindings stack))
+             interp-st))
+
+
+
+
+(define interp-st-decrement-reclimit (interp-st)
+  :guard (posp (interp-st->reclimit interp-st))
+  (update-interp-st->reclimit (1- (interp-st->reclimit interp-st)) interp-st))
+
+(define interp-st-increment-reclimit (interp-st)
+  (update-interp-st->reclimit (1+ (lnfix (interp-st->reclimit interp-st))) interp-st))
+
+(fty::defbitstruct gl-function-mode
+  ((dont-concrete-exec booleanp)
+   (dont-expand-def booleanp)
+   (dont-rewrite booleanp)
+   (dont-primitive-exec booleanp)))
+
+(define gl-function-mode-fix! (x)
+  :guard-hints(("Goal" :in-theory (enable gl-function-mode-fix)))
+  :enabled t
+  (mbe :logic (gl-function-mode-fix x)
+       :exec (loghead 4 (ifix x))))
+
+(define g-concretelist-p ((x gl-objectlist-p))
+  (if (atom x)
+      t
+    (and (gl-object-case (car x) :g-concrete)
+         (g-concretelist-p (Cdr x)))))
+
+(define g-concretelist-vals ((x gl-objectlist-p))
+  :guard (g-concretelist-p x)
+  :guard-hints (("goal" :in-theory (enable g-concretelist-p)))
+  (if (atom x)
+      nil
+    (cons (g-concrete->val (car x))
+          (g-concretelist-vals (cdr x)))))
+
+(define fncall-try-concrete-eval ((fn pseudo-fn-p)
+                                  (args gl-objectlist-p)
+                                  (dont-concrete-exec)
+                                  state)
+  :returns (mv ok ans)
+  (b* (((gl-function-mode mode))
+       ((when (or dont-concrete-exec
+                  (not (g-concretelist-p args))))
+        (mv nil nil))
+       ((mv err ans)
+        (magic-ev-fncall fn (g-concretelist-vals args) state t nil)))
+    (mv (not err) ans)))
+
+
+(def-b*-binder gl-interp-recursive-call
+  :body
+  `(b* (((mv . ,args)
+         (mbe :logic
+              (b* ((reclimit (interp-st->reclimit interp-st))
+                   ((mv . ,args) . ,forms)
+                   (interp-st (update-interp-st->reclimit reclimit interp-st)))
+                (mv . ,args))
+              :exec (progn$ . ,forms))))
+     ,rest-expr))
 
 
 (defines gl-interp
@@ -84,17 +259,19 @@
                           interp-st
                           state)
     ;; Translate a term to a GL object under the given alist substitution, preserving IFF.
-    :measure (list (pos-fix (interp-st->reclimit interp-st))
-                   12 0 0)
+    :measure (list (nfix (interp-st->reclimit interp-st))
+                   12 (pseudo-term-binding-count x) 0)
     :well-founded-relation acl2::nat-list-<
     :guard (bfr-listp (glcp-unify-alist-bfrlist alist) (interp-st->bfrstate interp-st))
-    (b* ((interp-st (interp-st-decrement-reclimit interp-st))
-         (current-equiv-contexts (interp-st->equiv-contexts interp-st))
+    :returns (mv err
+                 (xobj gl-object-p)
+                 new-interp-st
+                 new-state)
+    (b* ((current-equiv-contexts (interp-st->equiv-contexts interp-st))
          (interp-st (interp-st-update-equiv-contexts '(iff) interp-st))
-         ((mv err xobj interp-st state)
+         ((gl-interp-recursive-call err xobj interp-st state)
           (gl-interp-term-equivs x interp-st state))
          (interp-st (interp-st-update-equiv-contexts current-equiv-contexts interp-st))
-         (interp-st (interp-st-increment-reclimit interp-st))
          ((when err)
           (mv err nil interp-st state)))
       (simplify-if-test xobj interp-st state)))
@@ -102,10 +279,12 @@
   (define gl-interp-term-equivs ((x pseudo-termp)
                                  interp-st
                                  state)
-    :measure (list (interp-st->reclimit interp-st) 2020 (pseudo-term-count x) 40)
-    (b* (((when (zp (interp-st->reclimit interp-st)))
-          (glcp-interp-error "The recursion limit ran out."))
-         ((mv err xobj interp-st state)
+    :measure (list (nfix (interp-st->reclimit interp-st)) 2020 (pseudo-term-binding-count x) 40)
+    :returns (mv err
+                 (xobj gl-object-p)
+                 new-interp-st
+                 new-state)
+    (b* (((mv err xobj interp-st state)
           (gl-interp-term x interp-st state))
          ((when err) (mv err nil interp-st state))
          ((unless (glcp-term-obj-p xobj))
@@ -123,30 +302,188 @@
   (define gl-interp-term ((x pseudo-termp)
                           interp-st
                           state)
-    :measure (list (pos-fix (interp-st->reclimit interp-st))
-                   2020 (pseudo-term-count x) 20)
+    :measure (list (nfix (interp-st->reclimit interp-st))
+                   2020 (pseudo-term-binding-count x) 20)
+    :returns (mv err
+                 (xobj gl-object-p)
+                 new-interp-st
+                 new-state)
     (b* ((interp-st (interp-st-fix interp-st)))
       (pseudo-term-case x
         :const (glcp-value (g-concrete x.val))
-        :var (b* ((alist (interp-st->stack-top interp-st)))
-               (glcp-value (cdr (hons-assoc-equal x.name alist))))
+        :var (b* ((bindings (interp-st->bindings interp-st)))
+               (glcp-value (cdr (hons-assoc-equal x.name bindings))))
         :lambda
-        (b* (((mv bindings body) (cmr::lambda-nest-to-bindinglist x))
-             (interp-st (interp-st-duplicate-stack-top interp-st))
+        (b* (((mv x-bindings body) (lambda-nest-to-bindinglist x))
+             (interp-st (interp-st-dup-frame interp-st))
              (contexts (interp-st->equiv-contexts interp-st))
              (interp-st (update-interp-st->contexts nil interp-st))
-             ((mv err interp-st state)
+             ((gl-interp-recursive-call err interp-st state)
               ;; replaces the top of stack with the bindings
               (gl-interp-bindinglist bindings interp-st state))
              (interp-st (upate-interp-st->equiv-contexts contexts interp-st))
              ((when err)
-              (b* ((interp-st (interp-st-pop-stack interp-st)))
+              (b* ((interp-st (interp-st-pop-frame interp-st)))
                 (mv err nil interp-st state)))
              ((mv err val interp-st state)
               (gl-interp-term-equivs body interp-st state))
-             (interp-st (interp-st-pop-stack interp-st)))
+             (interp-st (interp-st-pop-frame interp-st)))
           (mv err val interp-st state))
         :fncall 
+        (b* (((when (and** (eq x.fn 'if) (eql (len x.args) 3)))
+              (gl-interp-if (first x.args)
+                            (second x.args)
+                            (third x.args)
+                            interp-st state))
+             ((when (and** (eq x.fn 'return-last) (eql (len x.args) 3)))
+              (gl-interp-return-last (first x.args)
+                                     (second x.args)
+                                     (third x.args)
+                                     interp-st state))
+             ((gl-interp-recursive-call err interp-st state)
+              (gl-interp-arglist x.args interp-st state))
+             ((when err)
+              (mv err nil interp-st state)))
+          (gl-interp-fncall x.fn (len x.args) interp-st state)))))
+
+  (define gl-interp-arglist ((args pseudo-term-listp)
+                             interp-st
+                             state)
+    :measure (list (nfix (interp-st->reclimit interp-st))
+                   2020 (pseudo-term-list-binding-count args) 20)
+    :returns (mv err
+                 new-interp-st
+                 new-state)
+    (b* (((when (atom args)) (mv nil interp-st state))
+         ((gl-interp-recursive-call err arg1 interp-st state)
+          (gl-interp-term-equivs (car args) interp-st state))
+         ((when err) (mv err interp-st state))
+         (interp-st (interp-st-push-scratch arg1 interp-st)))
+      (gl-interp-arglist (cdr args) interp-st state)))
+
+  (define gl-interp-bindinglist ((bindings bindinglist-p)
+                                 interp-st
+                                 state)
+    :measure (list (nfix (interp-st->reclimit interp-st))
+                   2020
+                   (bindinglist-count bindings)
+                   20)
+    :returns (mv err
+                 new-interp-st
+                 state)
+    (b* (((when (atom bindings)) (mv nil interp-st state))
+         ((binding x1) (car x))
+         ((gl-interp-recursive-call err interp-st state)
+          (gl-interp-arglist x1.args interp-st state))
+         ((when err) (mv err interp-st state))
+         (argslen (len x1.args))
+         (args (interp-st-peek-scratch argslen interp-st))
+         (interp-st (interp-st-pop-scratch argslen interp-st))
+         (interp-st (interp-st-add-bindings (pairlis$ x1.formals args) interp-st)))
+      (gl-interp-bindinglist (cdr bindings) interp-st state)))
+         
+  (define gl-interp-fncall ((fn pseudo-fnsym-p)
+                            (arity natp)
+                            interp-st
+                            state)
+    :measure (list (nfix (interp-st->reclimit interp-st))
+                   0 0 1)
+    (b* (((gl-function-mode fn-mode)
+          (gl-function-mode-fix!
+           (cdr (hons-assoc-equal fn (table-alist 'gl-fn-modes (w state))))))
+         (args (interp-st-peek-scratch arity interp-st))
+         (interp-st (interp-st-pop-scratch arity interp-st))
+         ((mv successp ans)
+          (fncall-try-concrete-eval fn args fn-mode.dont-concrete-exec state))
+         ((when successp)
+          (mv nil ans interp-st state))
+         ((gl-interp-recursive-call err successp ans interp-st state)
+          (gl-rewrite-fncall fn args fn-mode.dont-rewrite interp-st state))
+         ((when err)
+          (mv err nil interp-st state))
+         ((when successp)
+          (mv nil ans interp-st state))
+         ((mv successp ans interp-st state)
+          (gl-primitive-fncall fn args fn-mode.dont-primitive-exec interp-st state))
+         ((when successp)
+          (mv nil ans interp-st state))
+         ((mv err successp ans interp-st state)
+          (gl-interp-fn-definition fn args fn-mode.dont-expand-def interp-st state))
+         ((when err)
+          (mv err nil interp-st state))
+         ((when successp)
+          (mv nil ans interp-st state)))
+      (mv nil (g-apply fn args) interp-st state)))
+
+  (define gl-interp-fn-definition ((fn pseudo-fnsym-p)
+                                   (args gl-objectlist-p)
+                                   (dont)
+                                   interp-st
+                                   state)
+    :measure (list (nfix (interp-st->reclimit interp-st)) 0 0 0)
+    :returns (mv err successp
+                 (ans gl-object-p)
+                 new-interp-st
+                 new-state)
+    (b* (((when dont)
+          (mv nil nil nil interp-st state))
+         ((mv ok body formals)
+          (acl2::fn-get-def fn state))
+         ((unless ok)
+          (mv nil nil nil interp-st state))
+         ((unless (eql (len formals) arity))
+          (mv (gl-msg "Error interpreting a call of ~x0: it was given ~x1 arguments but has ~x2 formals."
+                   fn arity (len formals))
+              nil nil interp-st state))
+         ((when (zp (interp-st->reclimit interp-st)))
+          (mv (gl-msg "The recursion limit ran out.")
+              nil nil interp-st state))
+         (interp-st (interp-st-push-frame interp-st))
+         (interp-st (interp-st-set-bindings (pairlis$ formals args) interp-st))
+         (interp-st (interp-st-decrement-reclimit interp-st))
+         ((mv err ans interp-st state)
+          (gl-interp-term-equivs body interp-st state))
+         (interp-st (interp-st-pop-frame interp-st))
+         (interp-st (interp-st-increment-reclimit interp-st)))
+      (mv err ans interp-st state)))
+
+
+  (define gl-rewrite-fncall ((fn pseudo-fnsym-p)
+                             (args gl-objectlist-p)
+                             (dont)
+                             interp-st
+                             state)
+    :measure (list (nfix (interp-st->reclimit interp-st)) 0 0 0)
+    :returns (mv err successp
+                 (ans gl-object-p)
+                 new-interp-st
+                 new-state)
+    (b* (((when dont)
+          (mv nil nil nil interp-st state))
+         (backchain-limit (interp-st->backchain-limit interp-st))
+         ((when (eql 0 backchain-limit))
+          (mv nil nil nil interp-st state))
+         (interp-st (update-interp-st->backchain-limit (1- backchain-limit) interp-st))
+         (rules (fn-rewrite-rules fn (glcp-config->rewrite-rule-table
+                                      (interp-st->config interp-st))
+                                  (w state)))
+         ;; Pushes a stack frame if successful!
+         ((gl-interp-recursive-call err successp rhs interp-st state)
+          (gl-rewrite-fncall-rules rules fn args interp-st state))
+
+
+
+         
+
+              ((when (zp (interp-st->reclimit interp-st)))
+          (glcp-interp-error (gl-msg "The recursion limit ran out.")))
+         (interp-st (interp-st-decrement-reclimit interp-st))
+         
+         
+  gl-interp-if
+  gl-interp-return-last
+  gl-rewrite-fncall)
+             
         
          
     
